<?xml version="1.0"?>


<!DOCTYPE rdf:RDF [
    <!ENTITY terms "http://purl.org/dc/terms/" >
    <!ENTITY owl "http://www.w3.org/2002/07/owl#" >
    <!ENTITY obo "http://purl.obolibrary.org/obo/" >
    <!ENTITY dc "http://purl.org/dc/elements/1.1/" >
    <!ENTITY xsd "http://www.w3.org/2001/XMLSchema#" >
    <!ENTITY rdfs "http://www.w3.org/2000/01/rdf-schema#" >
    <!ENTITY rdf "http://www.w3.org/1999/02/22-rdf-syntax-ns#" >
]>


<rdf:RDF xmlns="http://www.semanticweb.org/engel/ontologies/2015/10/rdfBones#"
     xml:base="http://www.semanticweb.org/engel/ontologies/2015/10/rdfBones"
     xmlns:rdf="http://www.w3.org/1999/02/22-rdf-syntax-ns#"
     xmlns:terms="http://purl.org/dc/terms/"
     xmlns:owl="http://www.w3.org/2002/07/owl#"
     xmlns:xsd="http://www.w3.org/2001/XMLSchema#"
     xmlns:rdfs="http://www.w3.org/2000/01/rdf-schema#"
     xmlns:obo="http://purl.obolibrary.org/obo/"
     xmlns:dc="http://purl.org/dc/elements/1.1/">
    <owl:Ontology rdf:about="http://www.semanticweb.org/engel/ontologies/2015/10/rdfBones">
        <rdfs:comment xml:lang="en">This ontology models procedures, data and results from research involving materials from skeletal collections.</rdfs:comment>
        <owl:imports rdf:resource="http://vivoweb.org/ontology/core"/>
        <owl:versionIRI rdf:resource="http://www.semanticweb.org/engel/ontologies/2015/10/rdfBones/0.1"/>
    </owl:Ontology>
    


    <!-- 
    ///////////////////////////////////////////////////////////////////////////////////////
    //
    // Annotation properties
    //
    ///////////////////////////////////////////////////////////////////////////////////////
     -->

    


    <!-- http://purl.org/dc/elements/1.1/description -->

    <owl:AnnotationProperty rdf:about="&dc;description"/>
    


    <!-- http://purl.org/dc/terms/hasVersion -->

    <owl:AnnotationProperty rdf:about="&terms;hasVersion"/>
    


    <!-- 
    ///////////////////////////////////////////////////////////////////////////////////////
    //
    // Object Properties
    //
    ///////////////////////////////////////////////////////////////////////////////////////
     -->

    


    <!-- http://purl.obolibrary.org/obo/IAO_0000142 -->

    <rdf:Description rdf:about="&obo;IAO_0000142"/>
    


    <!-- http://purl.org/dc/terms/contributor -->

    <owl:ObjectProperty rdf:about="&terms;contributor">
        <rdfs:label>contributor</rdfs:label>
    </owl:ObjectProperty>
    


    <!-- http://purl.org/dc/terms/creator -->

    <owl:ObjectProperty rdf:about="&terms;creator">
        <rdfs:label xml:lang="en">Creator</rdfs:label>
        <rdfs:comment xml:lang="en">An entity primarily responsible for making the resource.</rdfs:comment>
        <terms:description xml:lang="en">Examples of a Creator include a person, an organization, or a service.</terms:description>
        <terms:hasVersion rdf:resource="http://dublincore.org/usage/terms/history/#creatorT-002"/>
        <rdfs:isDefinedBy rdf:resource="http://purl.org/dc/terms/"/>
        <rdfs:subPropertyOf rdf:resource="&terms;contributor"/>
        <rdfs:range rdf:resource="http://xmlns.com/foaf/0.1/Agent"/>
    </owl:ObjectProperty>
    


    <!-- http://purl.org/ontology/bibo/performer -->

    <rdf:Description rdf:about="http://purl.org/ontology/bibo/performer">
        <rdfs:subPropertyOf rdf:resource="&terms;contributor"/>
    </rdf:Description>
    


    <!-- http://purl.org/ontology/bibo/translator -->

    <rdf:Description rdf:about="http://purl.org/ontology/bibo/translator">
        <rdfs:subPropertyOf rdf:resource="&terms;contributor"/>
    </rdf:Description>
    


    <!-- http://www.semanticweb.org/engel/ontologies/2015/3/rdfBones#depicts -->

    <owl:ObjectProperty rdf:about="http://www.semanticweb.org/engel/ontologies/2015/3/rdfBones#depicts">
        <rdfs:label xml:lang="en">depicts</rdfs:label>
        <obo:IAO_0000115 xml:lang="en">An information source depicts something when it renders a representation of it, using words, sounds, images, or other means.</obo:IAO_0000115>
        <rdfs:comment xml:lang="en">The property is mainly applicable to images and audiovisual media, as obo:IAO_0000142 (&apos;mentions&apos;) covers cases were a textual information source denotes an entity.</rdfs:comment>
        <obo:IAO_0000119 xml:lang="en">https://en.wiktionary.org/wiki/depict, viewed on 19 October 2015.</obo:IAO_0000119>
        <rdfs:range rdf:resource="&obo;BFO_0000001"/>
        <rdfs:domain rdf:resource="&obo;IAO_0000030"/>
        <rdfs:subPropertyOf rdf:resource="&obo;IAO_0000136"/>
    </owl:ObjectProperty>
    


    <!-- http://www.semanticweb.org/engel/ontologies/2015/3/rdfBones#hasTranscription -->

    <owl:ObjectProperty rdf:about="http://www.semanticweb.org/engel/ontologies/2015/3/rdfBones#hasTranscription">
        <rdfs:label xml:lang="en">has transcription</rdfs:label>
        <obo:IAO_0000115 xml:lang="en">Relates a document to transcriptions of this document.</obo:IAO_0000115>
        <rdfs:domain rdf:resource="http://purl.org/ontology/bibo/Document"/>
        <rdfs:range rdf:resource="http://www.semanticweb.org/engel/ontologies/2015/3/rdfBones#Transcription"/>
    </owl:ObjectProperty>
    


    <!-- http://www.semanticweb.org/engel/ontologies/2015/3/rdfBones#isDepicted -->

    <owl:ObjectProperty rdf:about="http://www.semanticweb.org/engel/ontologies/2015/3/rdfBones#isDepicted">
        <rdfs:label xml:lang="en">is depicted in</rdfs:label>
        <obo:IAO_0000115 xml:lang="en">Something is depicted by an information source when the information source renders a representation of it, using words, sounds, images, or other means.</obo:IAO_0000115>
        <rdfs:comment xml:lang="en">The property is mainly applicable to images and audiovisual media, as rdfBones:isMentioned covers cases were an entity is denoted by a textual information source.</rdfs:comment>
        <obo:IAO_0000119 xml:lang="en">https://en.wiktionary.org/wiki/depict, viewed on 19 October 2015.</obo:IAO_0000119>
        <rdfs:domain rdf:resource="&obo;BFO_0000001"/>
        <rdfs:range rdf:resource="&obo;IAO_0000030"/>
        <rdfs:subPropertyOf rdf:resource="&obo;IAO_0000136"/>
        <owl:inverseOf rdf:resource="http://www.semanticweb.org/engel/ontologies/2015/3/rdfBones#depicts"/>
    </owl:ObjectProperty>
    


    <!-- http://www.semanticweb.org/engel/ontologies/2015/3/rdfBones#isMentioned -->

    <owl:ObjectProperty rdf:about="http://www.semanticweb.org/engel/ontologies/2015/3/rdfBones#isMentioned">
        <rdfs:label xml:lang="en">is mentioned in</rdfs:label>
        <obo:IAO_0000115 xml:lang="en">An entity E is mentioned by an information artifact IA exactly when IA has a component/part that denotes E.</obo:IAO_0000115>
        <rdfs:domain rdf:resource="&obo;BFO_0000001"/>
        <rdfs:range rdf:resource="&obo;IAO_0000030"/>
        <rdfs:subPropertyOf rdf:resource="&obo;IAO_0000136"/>
        <owl:inverseOf rdf:resource="&obo;IAO_0000142"/>
    </owl:ObjectProperty>
    


    <!-- http://www.semanticweb.org/engel/ontologies/2015/3/rdfBones#transcriptionOf -->

    <owl:ObjectProperty rdf:about="http://www.semanticweb.org/engel/ontologies/2015/3/rdfBones#transcriptionOf">
        <rdfs:label xml:lang="en">transcription of</rdfs:label>
        <obo:IAO_0000115 xml:lang="en">Relates a transcription to the original document.</obo:IAO_0000115>
        <rdfs:range rdf:resource="http://purl.org/ontology/bibo/Document"/>
        <rdfs:domain rdf:resource="http://www.semanticweb.org/engel/ontologies/2015/3/rdfBones#Transcription"/>
        <owl:inverseOf rdf:resource="http://www.semanticweb.org/engel/ontologies/2015/3/rdfBones#hasTranscription"/>
    </owl:ObjectProperty>
    


    <!-- 
    ///////////////////////////////////////////////////////////////////////////////////////
    //
    // Classes
    //
    ///////////////////////////////////////////////////////////////////////////////////////
     -->

    


    <!-- http://www.semanticweb.org/engel/ontologies/2015/3/rdfBones#ResearchNote -->

    <owl:Class rdf:about="http://www.semanticweb.org/engel/ontologies/2015/3/rdfBones#ResearchNote">
        <rdfs:label xml:lang="en">Research Note</rdfs:label>
        <rdfs:subClassOf>
            <owl:Restriction>
                <owl:onProperty rdf:resource="http://vivoweb.org/ontology/core#dateIssued"/>
                <owl:onClass rdf:resource="http://vivoweb.org/ontology/core#DateTimeValue"/>
                <owl:qualifiedCardinality rdf:datatype="&xsd;nonNegativeInteger">1</owl:qualifiedCardinality>
            </owl:Restriction>
        </rdfs:subClassOf>
        <rdfs:subClassOf>
            <owl:Restriction>
                <owl:onProperty rdf:resource="http://www.w3.org/2006/vcard/ns#note"/>
                <owl:qualifiedCardinality rdf:datatype="&xsd;nonNegativeInteger">1</owl:qualifiedCardinality>
                <owl:onDataRange rdf:resource="&xsd;string"/>
            </owl:Restriction>
        </rdfs:subClassOf>
        <rdfs:subClassOf>
            <owl:Restriction>
                <owl:onProperty rdf:resource="http://vivoweb.org/ontology/core#relates"/>
                <owl:onClass rdf:resource="&obo;BFO_0000001"/>
                <owl:minQualifiedCardinality rdf:datatype="&xsd;nonNegativeInteger">1</owl:minQualifiedCardinality>
            </owl:Restriction>
        </rdfs:subClassOf>
        <rdfs:subClassOf>
            <owl:Restriction>
                <owl:onProperty rdf:resource="&terms;creator"/>
                <owl:onClass rdf:resource="http://xmlns.com/foaf/0.1/Person"/>
                <owl:qualifiedCardinality rdf:datatype="&xsd;nonNegativeInteger">1</owl:qualifiedCardinality>
            </owl:Restriction>
        </rdfs:subClassOf>
        <obo:IAO_0000115 xml:lang="en">A piece of textual user input, containing additional information on one or several resources. It can be used to relate resources with each other.</obo:IAO_0000115>
    </owl:Class>
    


    <!-- http://www.semanticweb.org/engel/ontologies/2015/3/rdfBones#ResearchReference -->

    <owl:Class rdf:about="http://www.semanticweb.org/engel/ontologies/2015/3/rdfBones#ResearchReference">
        <rdfs:label xml:lang="en">Research Reference</rdfs:label>
        <rdfs:subClassOf rdf:resource="http://www.semanticweb.org/engel/ontologies/2015/3/rdfBones#ResearchNote"/>
        <rdfs:subClassOf>
            <owl:Restriction>
                <owl:onProperty rdf:resource="http://purl.org/ontology/bibo/pageEnd"/>
                <owl:maxCardinality rdf:datatype="&xsd;nonNegativeInteger">1</owl:maxCardinality>
            </owl:Restriction>
        </rdfs:subClassOf>
        <rdfs:subClassOf>
            <owl:Restriction>
                <owl:onProperty rdf:resource="http://purl.org/ontology/bibo/volume"/>
                <owl:maxCardinality rdf:datatype="&xsd;nonNegativeInteger">1</owl:maxCardinality>
            </owl:Restriction>
        </rdfs:subClassOf>
        <rdfs:subClassOf>
            <owl:Restriction>
                <owl:onProperty rdf:resource="http://vivoweb.org/ontology/core#relates"/>
                <owl:onClass rdf:resource="&obo;IAO_0000030"/>
                <owl:qualifiedCardinality rdf:datatype="&xsd;nonNegativeInteger">1</owl:qualifiedCardinality>
            </owl:Restriction>
        </rdfs:subClassOf>
        <rdfs:subClassOf>
            <owl:Restriction>
                <owl:onProperty rdf:resource="http://purl.org/ontology/bibo/pageStart"/>
                <owl:maxCardinality rdf:datatype="&xsd;nonNegativeInteger">1</owl:maxCardinality>
            </owl:Restriction>
        </rdfs:subClassOf>
        <rdfs:subClassOf>
            <owl:Restriction>
                <owl:onProperty rdf:resource="http://purl.org/ontology/bibo/chapter"/>
                <owl:maxCardinality rdf:datatype="&xsd;nonNegativeInteger">1</owl:maxCardinality>
            </owl:Restriction>
        </rdfs:subClassOf>
        <rdfs:subClassOf>
            <owl:Restriction>
                <owl:onProperty rdf:resource="http://purl.org/ontology/bibo/section"/>
                <owl:maxCardinality rdf:datatype="&xsd;nonNegativeInteger">1</owl:maxCardinality>
            </owl:Restriction>
        </rdfs:subClassOf>
        <obo:IAO_0000115 xml:lang="en">A piece of textual user input, creating a relationship between one or several entities and an information content entity or part of it.</obo:IAO_0000115>
    </owl:Class>
    


    <!-- http://www.semanticweb.org/engel/ontologies/2015/3/rdfBones#Transcription -->

    <owl:Class rdf:about="http://www.semanticweb.org/engel/ontologies/2015/3/rdfBones#Transcription">
        <rdfs:label>Transcription</rdfs:label>
        <rdfs:subClassOf rdf:resource="http://purl.org/ontology/bibo/Document"/>
        <obo:IAO_0000112 rdf:datatype="&xsd;string">&quot;Transcription turns handwritten and typed documents into searchable and machine-readable resources.&quot;
(https://transcription.si.edu/about; last accessed on 13 October 2015)</obo:IAO_0000112>
        <dc:description rdf:datatype="&xsd;string">The result of rendering a handwritten or recorded work in digital writing.</dc:description>
    </owl:Class>
</rdf:RDF>



<!-- Generated by the OWL API (version 3.5.1) http://owlapi.sourceforge.net -->

